New angle on encode vs decode, almost prove load for shared pts

src/high/crash_weakestpre.v
@@ -4,6 +4,7 @@ From iris.base_logic Require Import ghost_map.
 From Perennial.base_logic.lib Require Export ncfupd.
 From Perennial.program_logic Require crash_weakestpre.
 
+From self Require Import extra.
 From self.base Require Import primitive_laws class_instances.
 From self.high Require Export dprop resources lifted_modalities.
 
@@ -34,8 +35,10 @@ Section abs_history_lemmas.
     ℓ ↪[ abs_history_name ] abs_hist.
 
   Definition know_frag_history_loc ℓ (abs_hist : abs_history ST) : iProp Σ :=
-    own know_abs_history_name (◯ {[ ℓ := abs_hist_to_ra abs_hist ]}).
-    (* own abs_history_name ((◯ {[ ℓ := ◯ (abs_hist_to_ra abs_hist) ]}) : abs_historiesR). *)
+    ∃ enc,
+      ⌜(decode <$> enc = Some <$> abs_hist)⌝ ∗
+      own know_abs_history_name (◯ {[ ℓ := to_agree <$> enc ]}).
+      (* own abs_history_name ((◯ {[ ℓ := ◯ (abs_hist_to_ra abs_hist) ]}) : abs_historiesR). *)
 
   Lemma know_full_equiv ℓ abs_hist :
     know_full_history_loc ℓ abs_hist ⊣⊢ know_full_encoded_history_loc ℓ (encode <$> abs_hist).
@@ -96,10 +99,11 @@ Section abs_history_lemmas.
   Lemma own_frag_history_agree ℓ (part_hist : gmap time ST) hists :
     own_full_history hists -∗
     know_frag_history_loc ℓ part_hist -∗
-    ⌜∃ hist, hists !! ℓ = Some (hist) ∧ (encode <$> part_hist) ⊆ hist⌝.
+    ⌜∃ hist, hists !! ℓ = Some (hist) ∧ (Some <$> part_hist) ⊆ (decode <$> hist)⌝.
   Proof.
     rewrite /own_full_history.
-    iIntros "[O A] K".
+    iIntros "[O A]".
+    iDestruct 1 as (enc) "[%eq K]".
     iDestruct (own_valid_2 with "A K") as %[incl _]%auth_both_valid_discrete.
     apply singleton_included_l in incl.
     destruct incl as [hist' [look incl]].
@@ -108,75 +112,35 @@ Section abs_history_lemmas.
     simpl in look.
     iExists hist.
     iSplit; first done.
-    setoid_rewrite (inj_iff Some) in look.
+    rewrite <- eq.
     move: incl.
+    rewrite <- look.
     rewrite Some_included_total.
-    rewrite /abs_hist_to_ra.
-    rewrite -look.
-    rewrite map_fmap_compose.
-    rewrite lookup_included.
+    rewrite -to_agree_fmap.
     intros incl.
-    rewrite map_subseteq_spec.
-    iIntros (t enc lookPart).
-    specialize incl with t.
-    rewrite lookup_fmap in incl.
-    rewrite lookPart in incl.
-    simpl in incl.
-    rewrite lookup_fmap in incl.
-    apply option_included_total in incl.
-    destruct incl as [[=]|(? & ? & [=] & c & hih)].
-    rewrite -lookup_fmap in c.
-    apply lookup_fmap_Some in c.
-    destruct c as (? & ? & ?lookHist).
-    rewrite lookHist.
-    iPureIntro. f_equiv. subst.
-    apply to_agree_included in hih.
-    rewrite hih.
-    done.
+    iPureIntro.
+    by apply map_fmap_mono.
   Qed.
 
-  Lemma own_frag_history_agree_singleton ℓ t s hists :
+  Lemma own_frag_history_agree_singleton ℓ t (s : ST) hists :
     own_full_history hists -∗
     know_frag_history_loc ℓ {[ t := s ]} -∗
-    ⌜∃ hist, hists !! ℓ = Some (hist) ∧ hist !! t = Some (encode s)⌝.
+    ⌜∃ hist enc, hists !! ℓ = Some hist ∧ hist !! t = Some enc ∧ decode enc = Some s⌝.
   Proof.
     iIntros "H1 H2".
     iDestruct (own_frag_history_agree with "H1 H2") as %[hist [look H1]].
-    iExists hist. iPureIntro. split; [done|].
+    iExists hist. iPureIntro.
+    (* repeat split; [done| |]. *)
     (* elem_of *)
     rewrite map_fmap_singleton in H1.
     rewrite -> map_subseteq_spec in H1.
-    apply H1.
-    rewrite lookup_singleton.
-    done.
-  Qed.
-
-  Lemma own_full_history_alloc ℓ t (s : ST) hists hist :
-    hists !! ℓ = Some hist →
-    hist !! t = Some (encode s) →
-    own_full_history hists ==∗
-    own_full_history hists ∗ know_frag_history_loc ℓ {[ t := s ]}.
-  Proof.
-    rewrite /own_full_history.
-    iIntros (look lookHist) "[$ H2]".
-    iMod (own_update with "H2") as "[$ $]"; last done.
-    apply: auth_update_dfrac_alloc.
-    apply singleton_included_l.
-    eexists _.
-    rewrite lookup_fmap.
-    rewrite look.
-    simpl.
-    split; first reflexivity.
-    rewrite /abs_hist_to_ra.
-    apply Some_included_total.
-    rewrite map_fmap_compose.
-    rewrite !map_fmap_singleton.
-    apply singleton_included_l.
-    eexists _.
-    rewrite lookup_fmap.
-    rewrite lookHist.
-    simpl.
-    split; f_equiv.
+    specialize H1 with t (Some s).
+    epose proof (H1 _) as H2.
+    Unshelve. 2: { rewrite lookup_singleton. done. }
+    apply lookup_fmap_Some in H2.
+    destruct H2 as (enc & eq & lookHist).
+    exists enc.
+    repeat split; done.
   Qed.
 
   Lemma own_full_history_alloc' ℓ t encS (s : ST) hists hist :
@@ -186,26 +150,31 @@ Section abs_history_lemmas.
     own_full_history hists ==∗
     own_full_history hists ∗ know_frag_history_loc ℓ {[ t := s ]}.
   Proof.
-    rewrite /own_full_history.
     iIntros (look lookHist decEq) "[$ H2]".
-    iMod (own_update with "H2") as "[$ $]"; last done.
-    apply: auth_update_dfrac_alloc.
-    apply singleton_included_l.
-    eexists _.
-    rewrite lookup_fmap.
-    rewrite look.
-    simpl.
-    split; first reflexivity.
-    rewrite /abs_hist_to_ra.
-    apply Some_included_total.
-    rewrite map_fmap_compose.
+    rewrite /own_full_history /know_frag_history_loc.
+    iMod (own_update with "H2") as "[$ H]".
+    { apply (auth_update_dfrac_alloc _ _ {[ ℓ := {[ t := to_agree encS ]} ]}).
+      apply singleton_included_l.
+      eexists _.
+      rewrite lookup_fmap.
+      rewrite look.
+      simpl.
+      split; first reflexivity.
+      rewrite /abs_hist_to_ra.
+      apply Some_included_total.
+      (* rewrite map_fmap_compose. *)
+      (* rewrite !map_fmap_singleton. *)
+      apply singleton_included_l.
+      eexists _.
+      rewrite lookup_fmap.
+      rewrite lookHist.
+      simpl.
+      split; f_equiv. }
+    iExists {[ t := encS ]}.
     rewrite !map_fmap_singleton.
-    apply singleton_included_l.
-    eexists _.
-    rewrite lookup_fmap.
-    rewrite lookHist.
-    simpl.
-    split; f_equiv.
+    rewrite decEq.
+    iFrame.
+    done.
   Qed.
 
   (* This lemma seems false :'( *)
@@ -628,3 +597,4 @@ Section wpc.
   (*       iApply fupd_level_mask_intro_discard; [ set_solver+ | ]; iFrame. *)
   (* Qed. *)
 End wpc.
+
